Snapshot

code/hash/Hacl.SHA2Again.fst
@@ -7,6 +7,7 @@ module S = FStar.Seq
 module B = LowStar.Buffer
 module HS = FStar.HyperStack
 module ST = FStar.HyperStack.ST
+module D = FStar.Tactics.Derived
 
 friend Spec.SHA2Again
 
@@ -24,14 +25,31 @@ let k384_512 = B.gcmalloc_of_list HS.root C.k384_512_l
 let hashes a s l =
   Spec.hashes a s l
 
-let init a =
+let alloca a () =
   C.h224_reveal ();
   C.h256_reveal ();
   C.h384_reveal ();
   C.h512_reveal ();
+  [@ inline_let ]
   let l: list (word a) = Spec.(match a with
     | SHA2_224 -> C.h224_l
     | SHA2_256 -> C.h256_l
     | SHA2_384 -> C.h384_l
     | SHA2_512 -> C.h512_l) in
   B.alloca_of_list l
+
+let alloca_224 = D.specialize (alloca Spec.SHA2_224) []
+let alloca_256 = D.specialize (alloca Spec.SHA2_256) []
+let alloca_384 = D.specialize (alloca Spec.SHA2_384) []
+let alloca_512 = D.specialize (alloca Spec.SHA2_512) []
+
+let init a s =
+  let open Spec in
+  match a with
+  | SHA2_224 -> C.h224_reveal (); B.blit h224 0ul s 0ul 8ul
+  | _ -> admit ()
+
+let init_224 = D.specialize (init Spec.SHA2_224) []
+let init_256 = D.specialize (init Spec.SHA2_256) []
+let init_384 = D.specialize (init Spec.SHA2_384) []
+let init_512 = D.specialize (init Spec.SHA2_512) []
